\documentclass[../../Solutions.tex]{subfiles}
 
\begin{document}

\begin{itemize}
	\item [A.1]
		\begin{enumerate}[(a)]
			\item Multiplying the numerator and denominator by the complex conjugate produces the necessary simplification.
			$$ \frac{2-5i}{1+i}\frac{1-i}{1-i} = \frac{2-5i-2i-5}{1+1} = -\frac{3}{2}-\frac{7}{2}i $$
			\item We are able to show this equality simply by multiplying by $1$.
			$$ \frac{1}{i} = \frac{1}{i}\frac{i}{i} = \frac{i}{i^2} = \frac{i}{-1} = -i $$
		\end{enumerate}
	\item [A.2] For this exercise, we write $w = a+ib = Ae^{i\theta}$ and $z = c+id = Ce^{i\phi}$. This means $a = A\cos(\theta)$, $b = A\sin(\theta)$, $c = C\cos(\phi)$, and $d = C\sin(\phi)$.
		\begin{enumerate}[(a)]
			\item $\conj{(w+z)} = \conj{a+ib+c+id} = \conj{a+c+i(b+d)} = a+c-i(b+d) = a-ib+c-id = \conj{a+ib}+\conj{c+id} = \conj{w}+\conj{z}$
			\item $\conj{wz}=\conj{(a=ib)(c+id)}=\conj{ac-bd+i(ad+bc)}=ac-bd-i(ad+bc)=(a-ib)(c-id)=(\conj{a+ib})(\conj{c+id})=\conj{w}\conj{z}$
		\end{enumerate}
\end{itemize}

\end{document}